byteback-syntax/src/main/java/byteback/syntax/scene/encoder/SceneEncoder.java
@@ -1,0 +1,11 @@
+package byteback.syntax.scene.encoder;
+
+import byteback.syntax.encoder.Encoder;
+import byteback.syntax.printer.Printer;
+import soot.Scene;
+
+public interface SceneEncoder extends Encoder {
+
+    void encodeScene(Printer printer, Scene scene);
+
+}
