byteback-syntax/src/main/java/byteback/syntax/scene/encoder/to_bpl/SceneToBplEncoder.java
@@ -1,0 +1,53 @@
+package byteback.syntax.scene.encoder.to_bpl;
+
+import byteback.common.function.Lazy;
+import byteback.syntax.printer.Printer;
+import byteback.syntax.scene.encoder.SceneEncoder;
+import byteback.syntax.scene.type.declaration.encoder.to_bpl.ClassToBplEncoder;
+import soot.Scene;
+import soot.SootClass;
+
+import java.io.BufferedReader;
+import java.io.IOException;
+import java.io.InputStream;
+import java.io.InputStreamReader;
+
+public class SceneToBplEncoder implements SceneEncoder {
+
+    private static final Lazy<SceneToBplEncoder> INSTANCE = Lazy.from(SceneToBplEncoder::new);
+
+    public static SceneToBplEncoder v() {
+        return INSTANCE.get();
+    }
+
+    private SceneToBplEncoder() {
+    }
+
+    @Override
+    public void encodeScene(final Printer printer, final Scene scene) {
+        final String preludeResourcePath = "/boogie/ByteBackPrelude.bpl";
+
+        try (final InputStream preludeStream = getClass().getResourceAsStream(preludeResourcePath)) {
+            if (preludeStream == null) {
+                throw new IllegalStateException("Unable to find Boogie prelude.");
+            }
+
+            final var preludeStreamReader = new InputStreamReader(preludeStream);
+            final var preludeBufferedReader = new BufferedReader(preludeStreamReader);
+            String line;
+
+            while ((line = preludeBufferedReader.readLine()) != null) {
+                printer.printLine(line);
+            }
+        } catch (final IOException exception) {
+            throw new RuntimeException("Error opening the Boogie prelude.", exception);
+        }
+
+        for (final SootClass sootClass : scene.getClasses()) {
+            ClassToBplEncoder.v().encodeClass(printer, sootClass);
+        }
+
+        printer.close();
+    }
+
+}
