byteback-syntax/src/main/java/byteback/syntax/scene/type/declaration/encoder/to_bpl/ClassToBplEncoder.java
@@ -1,0 +1,69 @@
+package byteback.syntax.scene.type.declaration.encoder.to_bpl;
+
+import byteback.common.function.Lazy;
+import byteback.syntax.printer.Printer;
+import byteback.syntax.scene.type.declaration.encoder.ClassEncoder;
+import byteback.syntax.scene.type.declaration.member.method.body.value.encoder.to_bpl.ValueToBplEncoder;
+import byteback.syntax.scene.type.declaration.member.method.encoder.to_bpl.MethodToBplEncoder;
+import byteback.syntax.scene.type.declaration.tag.AxiomsProvider;
+import byteback.syntax.scene.type.declaration.tag.AxiomsTag;
+import soot.Hierarchy;
+import soot.SootClass;
+import soot.SootMethod;
+import soot.Value;
+
+import java.util.List;
+
+public class ClassToBplEncoder implements ClassEncoder {
+
+    private static final Lazy<ClassToBplEncoder> INSTANCE = Lazy.from(ClassToBplEncoder::new);
+
+    public static ClassToBplEncoder v() {
+        return INSTANCE.get();
+    }
+
+    private ClassToBplEncoder() {
+    }
+
+    public void encodeAxiom(final Printer printer, final Value axiomValue) {
+        printer.print("axiom ");
+        ValueToBplEncoder.v().encodeValue(printer, axiomValue);
+        printer.print(";");
+        printer.endLine();
+    }
+
+    public void encodeAxiomsTag(final Printer printer, final AxiomsTag axiomsTag) {
+        final List<Value> axiomValues = axiomsTag.getValues();
+
+        for (final Value axiomValue : axiomValues) {
+            encodeAxiom(printer, axiomValue);
+        }
+    }
+
+    public void encodeClassConstant(final Printer printer, final SootClass sootClass) {
+        printer.print("const unique `");
+        printer.print(sootClass.getName());
+        printer.print("`: Type;");
+        printer.endLine();
+    }
+
+    @Override
+    public void encodeClass(final Printer printer, final SootClass sootClass) {
+        printer.printLine("// START OF CLASS: " + sootClass.getName());
+        encodeClassConstant(printer, sootClass);
+        printer.endLine();
+        final AxiomsTag axiomsTag = AxiomsProvider.v().getOrCompute(sootClass);
+        encodeAxiomsTag(printer, axiomsTag);
+        printer.endLine();
+
+        if (sootClass.resolvingLevel() >= SootClass.SIGNATURES) {
+            for (final SootMethod sootMethod : sootClass.getMethods()) {
+                MethodToBplEncoder.v().encodeMethod(printer, sootMethod);
+            }
+        }
+
+        printer.printLine("// END OF CLASS: " + sootClass.getName());
+        printer.endLine();
+    }
+
+}
