byteback-syntax/src/main/java/byteback/syntax/scene/type/declaration/member/method/body/encoder/BodyEncoder.java
@@ -1,0 +1,11 @@
+package byteback.syntax.scene.type.declaration.member.method.body.encoder;
+
+import byteback.syntax.encoder.Encoder;
+import byteback.syntax.printer.Printer;
+import soot.Body;
+
+public interface BodyEncoder extends Encoder {
+
+    void encodeBody(final Printer printer, final Body body);
+
+}
