byteback-syntax/src/main/java/byteback/syntax/scene/type/declaration/member/method/body/encoder/to_bpl/BehaviorBodyToBplEncoder.java
@@ -1,0 +1,34 @@
+package byteback.syntax.scene.type.declaration.member.method.body.encoder.to_bpl;
+
+import byteback.common.function.Lazy;
+import byteback.syntax.printer.Printer;
+import byteback.syntax.scene.type.declaration.member.method.body.encoder.BodyEncoder;
+import byteback.syntax.scene.type.declaration.member.method.body.value.ReturnRef;
+import byteback.syntax.scene.type.declaration.member.method.body.value.encoder.to_bpl.ValueToBplEncoder;
+import soot.Body;
+import soot.Unit;
+import soot.Value;
+import soot.jimple.AssignStmt;
+
+public class BehaviorBodyToBplEncoder implements BodyEncoder {
+
+    private static final Lazy<BehaviorBodyToBplEncoder> INSTANCE = Lazy.from(BehaviorBodyToBplEncoder::new);
+
+    public static BehaviorBodyToBplEncoder v() {
+        return INSTANCE.get();
+    }
+
+    private BehaviorBodyToBplEncoder() {
+    }
+
+    @Override
+    public void encodeBody(final Printer printer, final Body body) {
+        for (final Unit unit : body.getUnits()) {
+            if (unit instanceof AssignStmt assignStmt && assignStmt.getLeftOp() instanceof ReturnRef) {
+                final Value behaviorValue = assignStmt.getRightOp();
+                ValueToBplEncoder.v().encodeValue(printer, behaviorValue);
+            }
+        }
+    }
+
+}
