byteback-syntax/src/main/java/byteback/syntax/scene/type/declaration/member/method/body/encoder/to_bpl/ProceduralBodyToBplEncoder.java
@@ -1,0 +1,23 @@
+package byteback.syntax.scene.type.declaration.member.method.body.encoder.to_bpl;
+
+import byteback.common.function.Lazy;
+import byteback.syntax.printer.Printer;
+import byteback.syntax.scene.type.declaration.member.method.body.encoder.BodyEncoder;
+import soot.Body;
+
+public class ProceduralBodyToBplEncoder implements BodyEncoder {
+
+    private static final Lazy<ProceduralBodyToBplEncoder> INSTANCE = Lazy.from(ProceduralBodyToBplEncoder::new);
+
+    public static ProceduralBodyToBplEncoder v() {
+        return INSTANCE.get();
+    }
+
+    private ProceduralBodyToBplEncoder() {
+    }
+
+    @Override
+    public void encodeBody(final Printer printer, final Body body) {
+    }
+
+}
