byteback-syntax/src/main/java/byteback/syntax/scene/type/declaration/member/method/body/tag/BehaviorFlagger.java
@@ -3,13 +3,14 @@ package byteback.syntax.scene.type.declaration.member.method.body.tag;
 import byteback.common.function.Lazy;
 import byteback.syntax.tag.TagFlagger;
 import soot.Body;
+import soot.SootMethod;
 
 /**
  * Flags the body of a method defining a Behavior expression.
  *
  * @author paganma
  */
-public class BehaviorFlagger extends TagFlagger<Body, BehaviorTag> {
+public class BehaviorFlagger extends TagFlagger<SootMethod, BehaviorTag> {
 
     private static final Lazy<BehaviorFlagger> INSTANCE =
             Lazy.from(() -> new BehaviorFlagger(BehaviorTag.v()));
