byteback-syntax/src/main/java/byteback/syntax/scene/type/declaration/member/method/body/value/NestedExpr.java
@@ -1,48 +1,63 @@
 package byteback.syntax.scene.type.declaration.member.method.body.value;
 
 import soot.*;
+import soot.jimple.internal.RValueBox;
 
+import java.util.ArrayList;
 import java.util.List;
 
 public class NestedExpr implements Immediate, DefaultCaseValue {
 
-    private final Value value;
+    private final RValueBox valueBox;
+
+    public NestedExpr(final RValueBox valueBox) {
+        this.valueBox = valueBox;
+    }
 
     public NestedExpr(final Value value) {
-        this.value = value;
+        this(new RValueBox(value));
     }
 
     public Value getValue() {
-        return value;
+        return valueBox.getValue();
     }
 
     @Override
     public List<ValueBox> getUseBoxes() {
-        return value.getUseBoxes();
+        final Value value = valueBox.getValue();
+        final var useBoxes = new ArrayList<ValueBox>(value.getUseBoxes());
+        useBoxes.add(valueBox);
+
+        return useBoxes;
     }
 
     @Override
     public Type getType() {
+        final Value value = valueBox.getValue();
         return value.getType();
     }
 
     @Override
     public Object clone() {
+        final Value value = valueBox.getValue();
         return new NestedExpr((Value) value.clone());
     }
 
     @Override
     public boolean equivTo(final Object object) {
+        final Value value = valueBox.getValue();
         return value.equivTo(object);
     }
 
     @Override
     public int equivHashCode() {
+        final Value value = valueBox.getValue();
         return value.equivHashCode();
     }
 
     @Override
     public void toString(final UnitPrinter printer) {
+        final Value value = valueBox.getValue();
         printer.literal("(");
         value.toString(printer);
         printer.literal(")");
