byteback-syntax/src/main/java/byteback/syntax/scene/type/declaration/member/method/body/value/encoder/to_bpl/ValueToBplEncoder.java
@@ -1,0 +1,217 @@
+package byteback.syntax.scene.type.declaration.member.method.body.value.encoder.to_bpl;
+
+import byteback.common.function.Lazy;
+import byteback.syntax.printer.Printer;
+import byteback.syntax.scene.type.declaration.member.method.body.value.*;
+import byteback.syntax.scene.type.declaration.member.method.body.value.analyzer.VimpTypeInterpreter;
+import byteback.syntax.scene.type.declaration.member.method.body.value.encoder.ValueEncoder;
+import byteback.syntax.scene.type.declaration.member.method.encoder.to_bpl.MethodToBplEncoder;
+import byteback.syntax.scene.type.encoder.to_bpl.TypeAccessToBplEncoder;
+import byteback.syntax.tag.AnnotationReader;
+import soot.*;
+import soot.jimple.*;
+import soot.util.Chain;
+
+import java.util.Arrays;
+import java.util.List;
+
+public class ValueToBplEncoder implements ValueEncoder {
+
+    private static final Lazy<ValueToBplEncoder> INSTANCE = Lazy.from(ValueToBplEncoder::new);
+
+    public static ValueToBplEncoder v() {
+        return INSTANCE.get();
+    }
+
+    private ValueToBplEncoder() {
+    }
+
+    public void encodeTypeConstant(final Printer printer, final TypeConstant typeConstant) {
+        printer.print("`");
+        printer.print(typeConstant.value.getClassName());
+        printer.print("`");
+    }
+
+    public void encodeFunction(final Printer printer, final String functionName, final Value... arguments) {
+        encodeFunction(printer, functionName, Arrays.stream(arguments).toList());
+    }
+
+    public void encodeFunction(final Printer printer, final String functionName, final Iterable<Value> arguments) {
+        printer.print(functionName);
+        printer.print("(");
+
+        printer.startItems(", ");
+        for (final Value value : arguments) {
+            printer.separate();
+            encodeValue(printer, value);
+        }
+        printer.endItems();
+        printer.print(")");
+    }
+
+    public void encodeBinding(final Printer printer, final Local binding) {
+        printer.print(binding.getName());
+        printer.print(": ");
+        final Type bindingType = binding.getType();
+        TypeAccessToBplEncoder.v().encodeTypeAccess(printer, bindingType);
+    }
+
+    public void encodeBindings(final Printer printer, final Iterable<Local> bindings) {
+        printer.startItems(", ");
+        for (final Local local : bindings) {
+            printer.separate();
+            encodeBinding(printer, local);
+        }
+        printer.endItems();
+    }
+
+    public void encodeQuantifierExpr(final Printer printer, final QuantifierExpr quantifierExpr) {
+        printer.print("(forall ");
+        final Chain<Local> bindings = quantifierExpr.getBindings();
+        encodeBindings(printer, bindings);
+        printer.print(" :: ");
+        final Value value = quantifierExpr.getValue();
+        encodeValue(printer, value);
+        printer.print(")");
+    }
+
+    public void encodeBinaryExpr(final Printer printer, final BinopExpr binopExpr, final String operator) {
+        printer.print("(");
+        final Value op1Value = binopExpr.getOp1();
+        encodeValue(printer, op1Value);
+        printer.print(operator);
+        final Value op2Value = binopExpr.getOp2();
+        encodeValue(printer, op2Value);
+        printer.print(")");
+    }
+
+    public void encodeLocal(final Printer printer, final Local local) {
+        printer.print(local.getName());
+    }
+
+    public void encodeArguments(final Printer printer, final List<Value> arguments) {
+        printer.startItems(", ");
+
+        for (final Value argument : arguments) {
+            printer.separate();
+            encodeValue(printer, argument);
+        }
+
+        printer.endItems();
+    }
+
+    public void encodeCallExpr(final Printer printer, final CallExpr callExpr) {
+        MethodToBplEncoder.v().encodeMethodName(printer, callExpr.getMethod());
+        printer.print("(");
+        encodeArguments(printer, callExpr.getArgs());
+        printer.print(")");
+    }
+
+    public void encodeDoubleConstant(final Printer printer, final DoubleConstant doubleConstant) {
+        if (Double.isFinite(doubleConstant.value)) {
+            printer.print(Double.toString(doubleConstant.value));
+        } else {
+            throw new IllegalArgumentException("Unable to encode NaN to Boogie");
+        }
+    }
+
+    public void encodeFloatConstant(final Printer printer, final FloatConstant floatConstant) {
+        if (Float.isFinite(floatConstant.value)) {
+            printer.print(Float.toString(floatConstant.value));
+        } else {
+            throw new IllegalArgumentException("Unable to encode NaN to Boogie");
+        }
+    }
+
+    @Override
+    public void encodeValue(final Printer printer, final Value value) {
+        System.out.println(value);
+        if (value instanceof final Immediate immediate) {
+            if (value instanceof Local local) {
+                encodeLocal(printer, local);
+                return;
+            }
+
+            if (immediate instanceof NestedExpr nestedExpr) {
+                encodeValue(printer, nestedExpr.getValue());
+                return;
+            }
+        }
+
+        if (value instanceof final ConcreteRef concreteRef) {
+            if (concreteRef instanceof ArrayRef arrayRef) {
+                encodeFunction(printer,"array.element", arrayRef.getBase(), arrayRef.getIndex());
+            }
+        }
+
+        if (value instanceof final Constant constant) {
+            if (constant instanceof final TypeConstant typeConstant) {
+                encodeTypeConstant(printer, typeConstant);
+                return;
+            }
+
+            if (constant instanceof final DoubleConstant doubleConstant) {
+                encodeDoubleConstant(printer, doubleConstant);
+                return;
+            }
+
+            if (constant instanceof final FloatConstant floatConstant) {
+                encodeFloatConstant(printer, floatConstant);
+                return;
+            }
+        }
+
+        if (value instanceof final BinopExpr binopExpr) {
+            if (binopExpr instanceof final ExtendsExpr extendsExpr) {
+                encodeFunction(printer, "type.extends", extendsExpr.getOp1(), extendsExpr.getOp2());
+                return;
+            }
+
+            if (binopExpr instanceof final ImpliesExpr impliesExpr) {
+                encodeBinaryExpr(printer, impliesExpr, " ==> ");
+                return;
+            }
+
+            if (binopExpr instanceof final AndExpr andExpr) {
+                final Type type = VimpTypeInterpreter.v().typeOf(andExpr);
+
+                if (type == BooleanType.v()) {
+                    encodeBinaryExpr(printer, andExpr, " && ");
+                    return;
+                }
+            }
+        }
+
+        if (value instanceof final UnopExpr unopExpr) {
+            if (unopExpr instanceof NegExpr negExpr) {
+                final Type type = VimpTypeInterpreter.v().typeOf(negExpr);
+
+                if (type == BooleanType.v()) {
+                    printer.print("!");
+                    encodeValue(printer, negExpr.getOp());
+                    return;
+                }
+            }
+
+            if (unopExpr instanceof LengthExpr lengthExpr) {
+                encodeFunction(printer, "array.lengthof", lengthExpr.getOp());
+                return;
+            }
+        }
+
+        if (value instanceof final InvokeExpr invokeExpr) {
+            if (invokeExpr instanceof final CallExpr callExpr) {
+                encodeCallExpr(printer, callExpr);
+                return;
+            }
+        }
+
+        if (value instanceof final QuantifierExpr quantifierExpr) {
+            encodeQuantifierExpr(printer, quantifierExpr);
+            return;
+        }
+
+        throw new IllegalStateException("Unable to convert value " + value + " of type " + value.getClass());
+    }
+
+}
