byteback-syntax/src/main/java/byteback/syntax/scene/type/declaration/member/method/encoder/MethodEncoder.java
@@ -1,0 +1,11 @@
+package byteback.syntax.scene.type.declaration.member.method.encoder;
+
+import byteback.syntax.encoder.Encoder;
+import byteback.syntax.printer.Printer;
+import soot.SootMethod;
+
+public interface MethodEncoder extends Encoder {
+
+    void encodeMethod(final Printer printer, final SootMethod sootMethod);
+
+}
