byteback-syntax/src/main/java/byteback/syntax/scene/type/declaration/member/method/encoder/to_bpl/BehaviorMethodToBplEncoder.java
@@ -1,0 +1,61 @@
+package byteback.syntax.scene.type.declaration.member.method.encoder.to_bpl;
+
+import byteback.common.function.Lazy;
+import byteback.syntax.encoder.Encoder;
+import byteback.syntax.name.BBLibNames;
+import byteback.syntax.printer.Printer;
+import byteback.syntax.scene.type.declaration.member.method.body.encoder.to_bpl.BehaviorBodyToBplEncoder;
+import byteback.syntax.scene.type.declaration.member.method.body.tag.TwoStateFlagger;
+import byteback.syntax.scene.type.declaration.member.method.body.value.encoder.to_bpl.ValueToBplEncoder;
+import byteback.syntax.scene.type.declaration.member.method.tag.ParameterLocalsProvider;
+import byteback.syntax.scene.type.encoder.to_bpl.TypeAccessToBplEncoder;
+import byteback.syntax.tag.AnnotationReader;
+import soot.Local;
+import soot.SootMethod;
+
+import java.util.List;
+
+public class BehaviorMethodToBplEncoder implements Encoder {
+
+    private static final Lazy<BehaviorMethodToBplEncoder> INSTANCE = Lazy.from(BehaviorMethodToBplEncoder::new);
+
+    public static BehaviorMethodToBplEncoder v() {
+        return INSTANCE.get();
+    }
+
+    private BehaviorMethodToBplEncoder() {
+    }
+
+    public void encodeBehaviorMethod(final Printer printer, final SootMethod sootMethod) {
+        if (!AnnotationReader.v().hasAnnotation(sootMethod, BBLibNames.PRELUDE_ANNOTATION)) {
+            printer.print("function `");
+            MethodToBplEncoder.v().encodeMethodName(printer, sootMethod);
+            printer.print("`(");
+
+            if (!AnnotationReader.v().hasAnnotation(sootMethod, BBLibNames.PRIMITIVE_ANNOTATION)) {
+                printer.print("h: Store, ");
+
+                if (TwoStateFlagger.v().isTagged(sootMethod.getActiveBody())) {
+                    printer.print("h': Store, ");
+                }
+            }
+
+            final List<Local> parameterLocals = ParameterLocalsProvider.v().getOrCompute(sootMethod).getValues();
+            ValueToBplEncoder.v().encodeBindings(printer, parameterLocals);
+
+            printer.print(") returns (");
+            TypeAccessToBplEncoder.v().encodeTypeAccess(printer, sootMethod.getReturnType());
+            printer.print(")");
+            printer.endLine();
+
+            printer.print("{ ");
+            if (sootMethod.hasActiveBody()) {
+                BehaviorBodyToBplEncoder.v().encodeBody(printer, sootMethod.getActiveBody());
+            }
+            printer.print(" }");
+
+            printer.endLine();
+        }
+    }
+
+}
