byteback-syntax/src/main/java/byteback/syntax/scene/type/declaration/member/method/encoder/to_bpl/MethodToBplEncoder.java
@@ -1,0 +1,52 @@
+package byteback.syntax.scene.type.declaration.member.method.encoder.to_bpl;
+
+import byteback.common.function.Lazy;
+import byteback.syntax.name.BBLibNames;
+import byteback.syntax.printer.Printer;
+import byteback.syntax.scene.type.declaration.member.method.encoder.MethodEncoder;
+import byteback.syntax.tag.AnnotationReader;
+import soot.ArrayType;
+import soot.SootMethod;
+import soot.Type;
+
+public class MethodToBplEncoder implements MethodEncoder {
+
+    private static final Lazy<MethodToBplEncoder> INSTANCE = Lazy.from(MethodToBplEncoder::new);
+
+    public static MethodToBplEncoder v() {
+        return INSTANCE.get();
+    }
+
+    private MethodToBplEncoder() {
+    }
+
+    public void encodeMethodName(final Printer printer, final SootMethod sootMethod) {
+        printer.print(sootMethod.getDeclaringClass().getName());
+        printer.print(".");
+        printer.print(sootMethod.getName());
+
+        printer.print("#");
+        printer.startItems("#");
+        for (final Type type : sootMethod.getParameterTypes()) {
+            printer.separate();
+            if (type instanceof ArrayType arrayType) {
+                printer.print(arrayType.baseType.toString());
+                printer.print("$");
+            } else {
+                printer.print(type.toString());
+            }
+        }
+        printer.endItems();
+        printer.print("#");
+    }
+
+    @Override
+    public void encodeMethod(final Printer printer, final SootMethod sootMethod) {
+        if (AnnotationReader.v().hasAnnotation(sootMethod, BBLibNames.BEHAVIOR_ANNOTATION)) {
+            BehaviorMethodToBplEncoder.v().encodeBehaviorMethod(printer, sootMethod);
+        } else {
+            ProceduralMethodToBplEncoder.v().encodeProceduralMethod(printer, sootMethod);
+        }
+    }
+
+}
