byteback-syntax/src/main/java/byteback/syntax/scene/type/declaration/member/method/encoder/to_bpl/ProceduralMethodToBplEncoder.java
@@ -1,0 +1,22 @@
+package byteback.syntax.scene.type.declaration.member.method.encoder.to_bpl;
+
+import byteback.common.function.Lazy;
+import byteback.syntax.encoder.Encoder;
+import byteback.syntax.printer.Printer;
+import soot.SootMethod;
+
+public class ProceduralMethodToBplEncoder implements Encoder {
+
+    private static final Lazy<ProceduralMethodToBplEncoder> INSTANCE = Lazy.from(ProceduralMethodToBplEncoder::new);
+
+    public static ProceduralMethodToBplEncoder v() {
+        return INSTANCE.get();
+    }
+
+    private ProceduralMethodToBplEncoder() {
+    }
+
+    public void encodeProceduralMethod(final Printer printer, final SootMethod sootMethod) {
+    }
+
+}
