byteback-syntax/src/main/java/byteback/syntax/scene/type/encoder/TypeAccessEncoder.java
@@ -1,0 +1,11 @@
+package byteback.syntax.scene.type.encoder;
+
+import byteback.syntax.printer.Printer;
+import soot.Scene;
+import soot.Type;
+
+public interface TypeAccessEncoder {
+
+    void encodeTypeAccess(final Printer printer, final Type type);
+
+}
