byteback-syntax/src/main/java/byteback/syntax/scene/type/encoder/to_bpl/TypeAccessToBplEncoder.java
@@ -1,0 +1,75 @@
+package byteback.syntax.scene.type.encoder.to_bpl;
+
+import byteback.common.function.Lazy;
+import byteback.syntax.printer.Printer;
+import byteback.syntax.scene.type.TypeType;
+import byteback.syntax.scene.type.encoder.TypeAccessEncoder;
+import soot.*;
+
+public class TypeAccessToBplEncoder implements TypeAccessEncoder {
+
+    private final static Lazy<TypeAccessToBplEncoder> INSTANCE = Lazy.from(TypeAccessToBplEncoder::new);
+
+    public static TypeAccessToBplEncoder v() {
+        return INSTANCE.get();
+    }
+
+    private TypeAccessToBplEncoder() {
+    }
+
+    @Override
+    public void encodeTypeAccess(final Printer printer, final Type type) {
+        if (type instanceof BooleanType) {
+            printer.print("bool");
+            return;
+        }
+
+        if (type instanceof ByteType) {
+            printer.print("`byte`");
+            return;
+        }
+
+        if (type instanceof ShortType) {
+            printer.print("`short`");
+            return;
+        }
+
+        if (type instanceof IntType) {
+            printer.print("`int`");
+            return;
+        }
+
+        if (type instanceof LongType) {
+            printer.print("`long`");
+            return;
+        }
+
+        if (type instanceof DoubleType) {
+            printer.print("`double`");
+            return;
+        }
+
+        if (type instanceof FloatType) {
+            printer.print("`float`");
+            return;
+        }
+
+        if (type instanceof RefType) {
+            printer.print("Reference");
+            return;
+        }
+
+        if (type instanceof ArrayType) {
+            printer.print("Reference");
+            return;
+        }
+
+        if (type instanceof TypeType) {
+            printer.print("Type");
+            return;
+        }
+
+        throw new IllegalStateException("Unable to encode type " + type);
+    }
+
+}
