byteback-syntax/src/main/java/byteback/syntax/tag/TagReader.java
@@ -44,7 +44,7 @@ public abstract class TagReader<K extends Host, V extends Tag> {
      * @param host The host to be queried.
      * @return `true` if the host contains the managed tag, `false` otherwise.
      */
-    public boolean isTagged(final Host host) {
+    public boolean isTagged(final K host) {
         return host.hasTag(tagName);
     }
 
